WIP decryption

fstar/new/MLS_Test_Internal.ml
@@ -1,9 +1,19 @@
 (* This file gets linked into the library for the purpose of doing an internal
    sanity test without having to link the test files. *)
 
+let dummy_data = List.map Char.code [ 'h'; 'e'; 'l'; 'l'; 'o' ]
+let dummy_user = List.map Char.code [ 'j'; 'o'; 'n'; 'a'; 't'; 'h'; 'a'; 'n' ]
+let dummy_group = List.map Char.code [ 'm'; 'y'; '_'; 'g'; 'r'; 'o'; 'u'; 'p' ]
+
+let dummy4 = [ 0; 1; 2; 3 ]
+
 let dummy32 =
-  [ 0; 1; 2; 3; 4; 5; 6; 7; 8; 9; 10; 11; 12; 13; 14; 15; 16 ] @
-  [ 0; 1; 2; 3; 4; 5; 6; 7; 8; 9; 10; 11; 12; 13; 14; 15; 16 ]
+  [ 0; 1; 2; 3; 4; 5; 6; 7; 8; 9; 10; 11; 12; 13; 14; 15 ] @
+  [ 0; 1; 2; 3; 4; 5; 6; 7; 8; 9; 10; 11; 12; 13; 14; 15 ]
+
+let dummy64 = dummy32 @ dummy32
+let dummy96 = dummy32 @ dummy32 @ dummy32
+let dummy128 = dummy64 @ dummy64
 
 let bytes_of_list l =
   FStar_Seq_Properties.seq_of_list (List.map (fun x ->
@@ -27,22 +37,63 @@ let debug_buffer s =
   Buffer.add_string buf "\n";
   Buffer.output_buffer stdout buf
 
+let debug_ascii s =
+  let buf = Buffer.create 1 in
+  List.iter (fun c -> Buffer.add_char buf (Char.chr c)) (list_of_bytes s);
+  Buffer.add_string buf "\n";
+  Buffer.output_buffer stdout buf
+
 let test () =
   let open MLS_Result in
+
+  print_endline "... brief unit test";
+  let dummy4 = bytes_of_list dummy4 in
   let dummy32 = bytes_of_list dummy32 in
+  let dummy64 = bytes_of_list dummy64 in
+  let dummy96 = bytes_of_list dummy96 in
+  let dummy128 = bytes_of_list dummy128 in
   let s = MLS_Crypto_Derived.derive_secret cs dummy32 dummy32 in
   match s with
   | Success s ->
       debug_buffer s;
       flush stdout;
   | _ ->
-      print_endline "Test 1 failed with *Error"; ;
-  let s = MLS.fresh_key_package dummy32 { signature_key = dummy32; identity = dummy32 } dummy32 in
+      failwith "Test 1 failed with *Error"; ;
+  let s = MLS.fresh_key_package dummy64 { signature_key = dummy32; identity = dummy32 } dummy32 in
   match s with
   | Success (s1, s2) ->
       debug_buffer s1;
       debug_buffer s2;
       flush stdout;
   | _ ->
-      print_endline "Test 2 failed with *Error"; ;
-  print_endline "Done with initial test"
+      failwith "Test 2 failed with *Error"; ;
+
+  (* High-level API test *)
+  print_endline "... high-level API test";
+  let pub, priv = match MLS.fresh_key_pair dummy32 with
+  | InternalError s -> failwith ("Internal error: " ^ s)
+  | ProtocolError s -> failwith ("Protocol error: " ^ s)
+  | Success (pub, priv) -> pub, priv
+  in
+  let cred = { MLS.identity = bytes_of_list dummy_user; signature_key = pub } in
+  let group_id = bytes_of_list dummy_group in
+  (* FIXME not enough entropy error if we use dummy96 even though signature says
+     so *)
+  let s = match MLS.create dummy128 cred priv group_id with
+  | InternalError s -> failwith ("Internal error: " ^ s)
+  | ProtocolError s -> failwith ("Protocol error: " ^ s)
+  | Success s -> s
+  in
+  let res = match MLS.send s dummy4 (bytes_of_list dummy_data) with
+  | InternalError s -> failwith ("Internal error: " ^ s)
+  | ProtocolError s -> failwith ("Protocol error: " ^ s)
+  | Success (s', (group_id, msg)) ->
+      MLS.process_group_message s' msg
+  in
+  match res with
+  | InternalError s -> failwith ("Internal error: " ^ s)
+  | ProtocolError s -> failwith ("Protocol error: " ^ s)
+  | Success (s'', MsgData data) ->
+      print_endline "... got data:";
+      debug_ascii data; ;
+  print_endline "... all good";
